src/Extraction/Compilerlib/Extraction.v
@@ -1,0 +1,6 @@
+From Stdlib Require Import Extraction 
+ExtrOcamlBasic ExtrOcamlNativeString
+ExtrOcamlZBigInt ExtrOcamlNatBigInt.
+From Compiler Require Import CompilerIns.
+Set Extraction Output Directory ".". 
+Separate Extraction CompilerIns.
